Finish verification of repl function (using cheated lemmas)

compiler/bootstrap/compilation/x64/64/proofs/replProofScript.sml
@@ -466,7 +466,7 @@ Inductive repl_types:
      repl_types (ffi,rs) (types,s,env) ∧
      infertype_prog types decs = Success new_types ∧
      evaluate$evaluate_decs s env decs = (new_s,Rval new_env) ⇒
-     repl_types (ffi,rs) (new_types,new_s,new_env)) ∧
+     repl_types (ffi,rs) (new_types,new_s,extend_dec_env new_env env)) ∧
 [repl_types_exn:]
   (∀ffi rs decs types new_types (s:'ffi state) env e new_s.
      repl_types (ffi,rs) (types,s,env) ∧
@@ -496,6 +496,9 @@ Definition ref_lookup_ok_def:
       (ty = Bool ⇒ v = Boolv T ∨ v = Boolv F) ∧
       (ty = Str ⇒ ∃t. v = Litv (StrLit t))
 End
+
+val _ = Parse.hide "types";
+val _ = Parse.hide "types_v";
 
 Theorem repl_types_thm:
   ∀(ffi:'ffi ffi_state) rs types s env.
@@ -534,9 +537,29 @@ Proof
   \\ fs [state_component_equality] *)
 QED
 
+Theorem repl_types_clock_refs_ffi:
+  repl_types (ffi,rs) (types,st with eval_state := NONE,env1) ⇒
+  repl_types (ffi,rs)
+    (types, st with <| clock := st.clock − ck;
+                       refs := st.refs ++ junk; ffi := st.ffi ;
+                       eval_state := NONE |>,env1)
+Proof
+  cheat (*
+  strip_tac
+  \\ drule repl_types_skip
+  \\ disch_then (qspecl_then [‘junk’,‘ck’,‘0’,‘0’] mp_tac)
+  \\ match_mp_tac (DECIDE “x = y ⇒ x ⇒ y”)
+  \\ rpt (AP_TERM_TAC ORELSE AP_THM_TAC)
+  \\ fs [state_component_equality] *)
+QED
+
+Definition the_Loc_def:
+  the_Loc (semanticPrimitives$Loc n) = n
+End
+
 Definition repl_rs_def:
-  repl_rs = [(Long "REPL" (Short "isEOF"),Bool,5:num);
-             (Long "REPL" (Short "nextString"),Str,6)]
+  repl_rs = [(Long "REPL" (Short "isEOF"),      Bool, the_Loc isEOF_loc);
+             (Long "REPL" (Short "nextString"), Str,  the_Loc nextString_loc)]
   (* TODO: fix loc numbers and add exn ref *)
 End
 
@@ -564,9 +587,6 @@ Proof
   cheat
 QED
 
-val _ = Parse.hide "types";
-val _ = Parse.hide "types_v";
-
 Theorem evaluate_repl:
   ∀(st:'ffi semanticPrimitives$state) s repl_str arg_str
    env s1_v types cur_gen next_id next_gen env1
@@ -581,7 +601,7 @@ Theorem evaluate_repl:
      LIST_TYPE AST_DEC_TYPE decs decs_v ∧
      INFER_INF_ENV_TYPE types types_v ∧
      STRING_TYPE input_str input_str_v ∧
-     (HOL_STRING_TYPE --> SUM_TYPE STRING_TYPE (LIST_TYPE AST_DEC_TYPE)) parse parse_v ∧
+     (STRING_TYPE --> SUM_TYPE STRING_TYPE (LIST_TYPE AST_DEC_TYPE)) parse parse_v ∧
      env_v = Conv NONE [Env env1 (env_id,0); Litv (IntLit (&env_id))] ∧
      conf_v = Conv NONE [s1_v; Litv (IntLit (&next_gen))] ∧
      repl_types (ffi,repl_rs) (types,st with eval_state := NONE,env1) ∧
@@ -592,7 +612,6 @@ Theorem evaluate_repl:
        evaluate st env [App Opapp [Var repl_str; Var arg_str]] = (s1,res) ∧
        res ≠ Rerr (Rabort Rtype_error)
 Proof
-
   strip_tac \\ completeInduct_on ‘st.clock’
   \\ rpt strip_tac \\ gvs [PULL_FORALL]
   (* expand App repl *)
@@ -781,7 +800,8 @@ Proof
   \\ simp [Once evaluate_def]
   \\ gvs [can_pmatch_all_def,pmatch_def,evaluate_Var,astTheory.pat_bindings_def]
   \\ CONV_TAC (DEPTH_CONV ml_progLib.nsLookup_conv) \\ simp [same_ctor_def]
-  \\ ‘repl_types (ffi,repl_rs) (new_types,st7 with eval_state := NONE,env2)’ by
+  \\ ‘repl_types (ffi,repl_rs)
+                 (new_types,st7 with eval_state := NONE, extend_dec_env env2 env1)’ by
    (irule repl_types_eval
     \\ drule check_and_tweak \\ strip_tac
     \\ first_assum $ irule_at (Pos hd)
@@ -797,7 +817,9 @@ Proof
   \\ IF_CASES_TAC \\ fs [dec_clock_def]
   \\ simp [Once evaluate_def,evaluate_Var,do_app_def]
   \\ ‘∃eof_n bv. isEOF_loc = Loc eof_n ∧
-       store_lookup eof_n st7.refs = SOME (Refv (Boolv bv))’ by cheat
+       store_lookup eof_n st7.refs = SOME (Refv (Boolv bv))’ by
+   (drule repl_types_thm \\ strip_tac \\ fs [repl_rs_def]
+    \\ fs [repl_moduleProgTheory.isEOF_def,the_Loc_def,ref_lookup_ok_def])
   \\ fs []
   (* evaluate if *)
   \\ rename [‘evaluate _ _ [If _ _ _]’]
@@ -805,10 +827,86 @@ Proof
   \\ IF_CASES_TAC THEN1 simp [evaluate_Con]
   \\ simp []
   (* let new_input = ... *)
-
-
-
-  \\ cheat
+  \\ simp [Once evaluate_def,evaluate_Var]
+  \\ simp [Once evaluate_def,evaluate_Var,evaluate_list]
+  \\ CONV_TAC (DEPTH_CONV ml_progLib.nsLookup_conv) \\ simp [same_ctor_def]
+  (* evaluating !REPL.nextString *)
+  \\ simp [mlbasicsProgTheory.deref_v_def,do_opapp_def]
+  \\ IF_CASES_TAC \\ fs [dec_clock_def]
+  \\ simp [Once evaluate_def,evaluate_Var,do_app_def]
+  \\ ‘∃next_n inp. nextString_loc = Loc next_n ∧
+       store_lookup next_n st7.refs = SOME (Refv (Litv (StrLit inp)))’ by
+   (drule repl_types_thm \\ strip_tac \\ fs [repl_rs_def]
+    \\ fs [repl_moduleProgTheory.nextString_def,the_Loc_def,ref_lookup_ok_def])
+  \\ fs []
+  \\ ‘STRING_TYPE (strlit inp) (Litv (StrLit inp))’ by fs [STRING_TYPE_def]
+  (* calling parse *)
+  \\ simp [Once evaluate_def,evaluate_Var]
+  \\ simp [Once evaluate_def,evaluate_Var,evaluate_list]
+  \\ simp [evaluate_Var,namespaceTheory.nsOptBind_def]
+  \\ CONV_TAC (DEPTH_CONV ml_progLib.nsLookup_conv) \\ simp [same_ctor_def]
+  \\ qpat_x_assum ‘(STRING_TYPE --> _) _ parse_v’ mp_tac
+  \\ strip_tac
+  \\ drule_all Arrow_IMP
+  \\ fs [dec_clock_def]
+  \\ qmatch_goalsub_abbrev_tac ‘(st2, Rerr (Rabort Rtimeout_error))’
+  \\ disch_then (qspec_then ‘(st2 with clock := st2.clock − 1)’ strip_assume_tac)
+  \\ fs [] \\ IF_CASES_TAC \\ fs [Abbr‘st2’,dec_clock_def]
+  \\ Cases_on ‘res = Rerr (Rabort Rtimeout_error)’ \\ gvs []
+  (* case on result of parse *)
+  \\ Cases_on ‘parse' (strlit inp)’ \\ gvs [std_preludeTheory.SUM_TYPE_def]
+  THEN1
+   (rename [‘_ = INL msg’]
+    \\ simp [Once evaluate_def,evaluate_Var]
+    \\ gvs [can_pmatch_all_def,pmatch_def,evaluate_Var]
+    \\ CONV_TAC (DEPTH_CONV ml_progLib.nsLookup_conv) \\ simp [same_ctor_def]
+    \\ simp [Once evaluate_def]
+    \\ gvs [can_pmatch_all_def,pmatch_def,evaluate_Var,astTheory.pat_bindings_def]
+    \\ CONV_TAC (DEPTH_CONV ml_progLib.nsLookup_conv) \\ simp [same_ctor_def]
+    (* call report_error *)
+    \\ simp [Once evaluate_def,evaluate_Var,evaluate_Con,evaluate_list,
+             namespaceTheory.nsOptBind_def]
+    \\ CONV_TAC (DEPTH_CONV ml_progLib.nsLookup_conv) \\ simp [same_ctor_def]
+    \\ unabbrev_all_tac
+    \\ assume_tac compiler64prog_report_error_v_thm
+    \\ drule_all Arrow_IMP
+    \\ simp [Once evaluate_def,evaluate_Var,evaluate_list]
+    \\ simp [evaluate_Var,namespaceTheory.nsOptBind_def]
+    \\ CONV_TAC (DEPTH_CONV ml_progLib.nsLookup_conv) \\ simp [same_ctor_def]
+    \\ qmatch_goalsub_abbrev_tac ‘(st2, Rerr (Rabort Rtimeout_error))’
+    \\ disch_then (qspec_then ‘dec_clock st2’ strip_assume_tac) \\ fs []
+    \\ fs [] \\ IF_CASES_TAC \\ fs []
+    \\ Cases_on ‘res = Rerr (Rabort Rtimeout_error)’ \\ gvs [dec_clock_def]
+    \\ simp [Once evaluate_def,evaluate_Var,evaluate_Con,evaluate_list,
+             namespaceTheory.nsOptBind_def,evaluate_Lit]
+    (* recursive call *)
+    \\ last_x_assum irule \\ gvs [Abbr‘st2’]
+    \\ drule evaluate_clock_decs \\ strip_tac \\ fs []
+    \\ conj_tac THEN1 rewrite_tac [GSYM repl_v_def]
+    \\ rpt (first_assum $ irule_at Any)
+    \\ rewrite_tac [GSYM APPEND_ASSOC,integerTheory.INT_ADD_CALCULATE]
+    \\ irule repl_types_clock_refs_ffi \\ fs [])
+  (* parse is successful *)
+  \\ rename [‘_ = INR new_decs’]
+  \\ simp [Once evaluate_def,evaluate_Var]
+  \\ gvs [can_pmatch_all_def,pmatch_def,evaluate_Var]
+  \\ CONV_TAC (DEPTH_CONV ml_progLib.nsLookup_conv) \\ simp [same_ctor_def]
+  \\ simp [Once evaluate_def]
+  \\ gvs [can_pmatch_all_def,pmatch_def,evaluate_Var,astTheory.pat_bindings_def]
+  \\ CONV_TAC (DEPTH_CONV ml_progLib.nsLookup_conv) \\ simp [same_ctor_def]
+  \\ simp [Once evaluate_def]
+  \\ gvs [can_pmatch_all_def,pmatch_def,evaluate_Var,astTheory.pat_bindings_def]
+  \\ CONV_TAC (DEPTH_CONV ml_progLib.nsLookup_conv) \\ simp [same_ctor_def]
+  \\ simp [Once evaluate_def,evaluate_Var,evaluate_Con,evaluate_list,
+           namespaceTheory.nsOptBind_def,evaluate_Lit]
+  (* recursive call *)
+  \\ last_x_assum irule
+  \\ drule evaluate_clock_decs \\ strip_tac \\ fs []
+  \\ unabbrev_all_tac \\ fs []
+  \\ conj_tac THEN1 rewrite_tac [GSYM repl_v_def]
+  \\ rpt (first_assum $ irule_at Any)
+  \\ rewrite_tac [GSYM APPEND_ASSOC,integerTheory.INT_ADD_CALCULATE]
+  \\ irule repl_types_clock_refs_ffi \\ fs []
 QED
 
 (*
